src/linear/impl/ArrayListImpl.dfy
@@ -1,50 +1,40 @@
-include "../../../src/linear/impl/ArrayList.dfy"
+include "../../Utils.dfy"
+include "ArrayList.dfy"
 
-
-class ArrayListIteratorImpl extends ArrayListIterator {
+class ArrayListIteratorImpl extends ListIterator {
   var parent: ArrayListImpl
-  var node: nat;//el indice exterior--corresponde a (parent.c+node)%parent.list.Length
+  var index: nat
 
   predicate Valid()
     reads this, parent, parent.Repr()
   {
-    && parent.Valid()
-    && 0<=node<=parent.nelems
+    parent.Valid()
+    && 0 <= index <= parent.size
   }
 
-  function Parent(): ArrayList
+  function Parent(): List
     reads this
   {
     parent
   }
 
-  function Index(): nat
+  function Index() : nat
     reads this, parent, parent.Repr()
     requires Valid()
     requires Parent().Valid()
     ensures Index() <= |Parent().Model()|
   {
-    node
+    index
   }
 
-  constructor(l: ArrayListImpl)
-    requires l.Valid()
+  constructor(vector: ArrayListImpl)
+    requires vector.Valid()
     ensures Valid()
-    ensures parent == l
+    ensures Parent() == vector
     ensures Index() == 0
   {
-    parent := l;
-    node := 0;
-  }
-
-  constructor CopyCtr(it: ArrayListIteratorImpl)
-    requires it.Valid()
-    ensures Valid()
-    ensures parent == it.parent
-    ensures node == it.node
-  {
-    parent := it.parent;
-    node := it.node;
+    this.parent := vector;
+    this.index := 0;
   }
 
   function method HasNext(): bool
@@ -53,32 +43,7 @@ class ArrayListIteratorImpl extends ArrayListIterator {
     requires Parent().Valid()
     ensures HasNext() <==> Index() < |Parent().Model()|
   {
-    node < parent.nelems
-  }
-
-  method Next() returns (x: int)
-    modifies this
-    requires Valid()
-    requires Parent().Valid()
-    requires HasNext()
-    requires allocated(Parent())
-   //requires forall it | it in Parent().Iterators() :: allocated(it)
-    ensures Parent().Valid()
-    ensures Valid()
-    ensures old(Index()) < Index()
-    ensures old(Parent()) == Parent()
-    ensures old(Index()) < |Parent().Model()|
-    ensures old(Parent().Model()) == Parent().Model()
-    ensures Parent().Iterators() == old(Parent().Iterators())
-    ensures x == Parent().Model()[old(Index())]
-    ensures Index() == 1 + old(Index())
-    ensures forall it | it in Parent().Iterators() && old(it.Valid()) ::
-      it.Valid() && (it != this ==> it.Index() == old(it.Index()))
-    ensures forall x | x in Parent().Repr() - old(Parent().Repr()) :: fresh(x)
-    ensures forall x | x in Parent().Repr() :: allocated(x)
-  {parent.modelIndex(parent.list,parent.c,parent.nelems);
-    x := parent.list[(parent.c+node)%parent.list.Length];
-    node := node+1;
+    index < parent.size
   }
 
   function method Peek(): int
@@ -87,11 +52,38 @@ class ArrayListIteratorImpl extends ArrayListIterator {
     requires Parent().Valid()
     requires HasNext()
     ensures Peek() == Parent().Model()[Index()]
-  { parent.modelIndex(parent.list,parent.c,parent.nelems);
-    parent.list[(parent.c+node)%parent.list.Length]
+  {
+    parent.elements[index]
   }
 
-  method Copy() returns (it: ArrayListIterator)
+  method Next() returns (x: int)
+    modifies this
+    requires Valid()
+    requires Parent().Valid()
+    requires HasNext()
+    requires allocated(Parent())
+    requires forall it | it in Parent().Repr() :: allocated(it)
+    ensures Parent().Valid()
+    ensures Valid()
+    ensures old(Parent()) == Parent()
+    ensures old(Parent().Model()) == Parent().Model()       // ?
+
+    ensures forall x {:trigger x in Parent().Repr(), x in old(Parent().Repr())} | x in Parent().Repr() - old(Parent().Repr()) :: fresh(x)
+    ensures fresh(Parent().Repr() - old(Parent().Repr()))
+    ensures forall x | x in Parent().Repr() :: allocated(x)
+
+    ensures Parent().Iterators() == old(Parent().Iterators())   // ?
+    ensures x == Parent().Model()[old(Index())]
+    ensures Index() == 1 + old(Index())
+    ensures forall it | it in Parent().Iterators() && old(it.Valid()) ::
+       it.Valid() && (it != this ==> it.Index() == old(it.Index()))
+    {
+      var elem := parent.elements[index];
+      index := index + 1;
+      return elem;
+    }
+
+  method Copy() returns (it: ListIterator)
     modifies Parent(), Parent().Repr()
     requires Valid()
     requires Parent().Valid()
@@ -99,32 +91,65 @@ class ArrayListIteratorImpl extends ArrayListIterator {
     requires forall it | it in Parent().Iterators() :: allocated(it)
     ensures fresh(it)
     ensures Valid()
-    ensures it.Valid()
-    ensures Parent().Valid()
-    ensures it in Parent().Iterators()
-    ensures Parent().Iterators() == {it} + old(Parent().Iterators())
     ensures Parent() == old(Parent())
+    ensures Parent().Valid()
+    ensures Parent().Model() == old(Parent().Model())
+
+    ensures forall x {:trigger x in Parent().Repr(), x in old(Parent().Repr())} | x in Parent().Repr() - old(Parent().Repr()) :: fresh(x)
+    ensures fresh(Parent().Repr()-old(Parent().Repr()))
+    ensures forall x | x in Parent().Repr() :: allocated(x)
+    
+    ensures it.Valid()
+    ensures Parent().Iterators() == {it} + old(Parent().Iterators())
     ensures Parent() == it.Parent()
     ensures Index() == it.Index()
-    ensures it.Valid()
     ensures forall it | it in old(Parent().Iterators()) && old(it.Valid()) ::
       it.Valid() && it.Index() == old(it.Index())
-    ensures Parent().Model() == old(Parent().Model())
-    ensures forall x | x in Parent().Repr() - old(Parent().Repr()) :: fresh(x)
+    {
+      var itImpl := new ArrayListIteratorImpl(parent);      
+      itImpl.index := index;
+      it := itImpl; 
+      parent.iterators := parent.iterators + { itImpl };
+    }
+
+  method Set(x: int)
+    modifies Parent(), Parent().Repr()
+    requires Valid()
+    requires Parent().Valid()
+    requires allocated(Parent())
+    requires forall it | it in Parent().Repr() :: allocated(it)
+    requires HasNext()
+    ensures Valid()
+    ensures Parent().Valid()
+    ensures Parent() == old(Parent())
+    ensures |Parent().Model()| == old(|Parent().Model()|)
+    ensures Parent().Model()[old(Index())] == x
+    ensures forall i | 0 <= i < |Parent().Model()| && i != old(Index()) ::
+      Parent().Model()[i] == old(Parent().Model()[i])
+
+    ensures forall x {:trigger x in Parent().Repr(), x in old(Parent().Repr())} | x in Parent().Repr() - old(Parent().Repr()) :: fresh(x)
+    ensures fresh(Parent().Repr()-old(Parent().Repr()))
     ensures forall x | x in Parent().Repr() :: allocated(x)
-  {
-    it := new ArrayListIteratorImpl.CopyCtr(this);
-    parent.iters := {it} + parent.iters;
+
+    //ensures Index() == old(Index())
+    ensures Parent().Iterators() == old(Parent().Iterators())
+    ensures forall it | it in old(Parent().Iterators()) && old(it.Valid()) ::
+      it.Valid() && it.Index() == old(it.Index())
+ {
+    parent.elements[index] := x;
   }
 }
+
+
 class ArrayListImpl extends ArrayList {
-  var list: array<int>;
-  var c: nat;
-  var nelems: nat;
-  var iters: set<ArrayListIteratorImpl>;
+  var elements: array<int>;
+  var size: nat;
+  ghost var iterators: set<ArrayListIteratorImpl>
+
+  lemma UselessLemma()
+    ensures Repr() == ReprFamily(ReprDepth());
 
   function ReprDepth(): nat
-    ensures ReprDepth() > 0
   {
     1
   }
@@ -132,7 +157,7 @@ class ArrayListImpl extends ArrayList {
   function Repr0(): set<object>
     reads this
   {
-    {this, list}+iters
+    {this, elements} + iterators
   }
 
   function ReprFamily(n: nat): set<object>
@@ -147,322 +172,240 @@ class ArrayListImpl extends ArrayList {
       ReprFamily(n-1)
   }
 
-  lemma UselessLemma()
-    ensures Repr() == ReprFamily(ReprDepth());
-  {}
-
-  function method Size(): nat
-    reads this, Repr()
-    requires Valid()
-    ensures Size() == |Model()|
-  {
-     nelems
-  }
-
   predicate Valid()
     reads this, Repr()
   {
-    0 <= c < list.Length && 0 <= nelems <= list.Length
-    && forall it | it in iters :: it.parent == this && {it} !! {this,list}
-
+    0 <= size <= elements.Length
+      && elements.Length >= 1
+      && forall it | it in iterators :: it.parent == this
   }
 
-  function Model(): seq<int> // Los elementos estan en [c..(c+nelems)%Length) circularmente
+  function Model(): seq<int>
     reads this, Repr()
     requires Valid()
   {
-    ModelAux(list,c,nelems)
+    elements[..size]
   }
 
-  function ModelAux(a:array<int>,c:nat,nelems:nat):seq<int>
-    reads a
-    requires 0 <= c < a.Length && 0 <= nelems <= a.Length
-    ensures |ModelAux(a,c,nelems)|==nelems
-  {
-    if nelems == 0 then
-      []
-    else if c + nelems <= a.Length then
-      a[c..c+nelems]
-    else
-      a[c..a.Length] + a[0..(c+nelems)%a.Length]
-  }
-
-lemma modelIndexAux(a:array<int>,c:nat,nelems:nat,k:nat)
-    requires 0 <= c < a.Length && 0 <= nelems <= a.Length
-    requires 0<=k<nelems
-    ensures ModelAux(a,c,nelems)[k]==a[(c+k)%a.Length]
-{ modulo(c+k,a.Length);
-  assert c+k<a.Length ==> ModelAux(a,c,nelems)[k]==a[(c+k)];
-  assume c+k>=a.Length ==> ModelAux(a,c,nelems)[k]==a[(c+k)%a.Length];
-}
-
-lemma modelIndex(a:array<int>,c:nat,nelems:nat)
-    requires 0 <= c < a.Length && 0 <= nelems <= a.Length
-    ensures forall k| 0<=k<nelems ::  ModelAux(a,c,nelems)[k]==a[(c+k)%a.Length]
-{
-forall k| 0<=k<nelems
-  ensures ModelAux(a,c,nelems)[k]==a[(c+k)%a.Length]
-  {modelIndexAux(a,c,nelems,k);}
-
-
-}
-
-  lemma incDeque(a:array<int>,c:nat,nelems:nat)
-    requires 0<=c<a.Length &&0<nelems<=a.Length
-    ensures ModelAux(a,c,nelems)==[a[c]]+ModelAux(a,(c+1)%a.Length,nelems-1)
-  {
-    if c + 1 < a.Length {
-      assert ModelAux(a,c,nelems)==[a[c]]+ModelAux(a,(c+1),nelems-1);
-      assert (c+1)%a.Length==c+1;
-    }
-  }
-
-  lemma incEnque(a:array<int>,c:nat,nelems:nat)
-    requires 0 <= c < a.Length && 0 <= nelems < a.Length
-    ensures ModelAux(a, c, nelems+1) == ModelAux(a, c, nelems) + [a[(c+nelems)%a.Length]]
-  {
-    if c + nelems < a.Length { // consecutive nelems+1 elements [c..c+nelems]
-      assert ModelAux(a, c, nelems+1)
-        == ModelAux(a, c, nelems) + [a[(c+nelems)%a.Length]];
-    } else { //elements [c..a.Length] followed by [0..(c+nelems+1)%a.Length]
-      assert c+nelems+1 > a.Length && ((c+nelems+1)%a.Length)
-        == (c+nelems) % a.Length+1;
-      assert a[c..a.Length] + a[0..(c+nelems+1)%a.Length]
-        == a[c..a.Length]+a[0..(c+nelems)%a.Length]+[a[(c+nelems)%a.Length]];
-    }
-  }
-
-
-function Iterators(): set<ArrayListIterator>
+  function Iterators(): set<ListIterator>
     reads this, Repr()
     requires Valid()
     ensures forall it | it in Iterators() :: it in Repr() && it.Parent() == this
-    {
-      iters
-
-     }
-
-  method Begin() returns (it: ArrayListIterator)
-    modifies this, Repr()
-    requires Valid()
-    requires forall it | it in Iterators() :: allocated(it)
-    ensures Valid()
-    ensures Model() == old(Model())
-    ensures fresh(it)
-    ensures Iterators() == {it} + old(Iterators())
-    ensures it.Valid()
-    ensures it.Index() == 0
-    ensures it.Parent() == this
-    ensures forall it | it in old(Iterators()) && old(it.Valid()) ::
-      it.Valid() && it.Index() == old(it.Index())
-    ensures forall x | x in Repr() - old(Repr()) :: fresh(x)
-    ensures forall x | x in Repr() :: allocated(x)
-
-    {
-      it:=new ArrayListIteratorImpl(this);
-      iters:={it}+iters;
-
-    }
-
-  function method Empty(): bool
-    reads this, Repr()
-    requires Valid()
-    ensures Empty() <==> Model() == []
   {
-    nelems == 0
+    iterators
   }
+
 
   constructor()
     ensures Valid()
     ensures Model() == []
     ensures fresh(Repr())
   {
-    list := new int[10];
-    c:=0;
-    nelems:=0;
-    iters:={};
+    elements := new int[1];
+    size := 0;
+    iterators := {};
   }
 
- 
-  // Auxiliary method to duplicate space
-  method grow()
-    modifies Repr()
+  function method Empty(): bool
+    reads this, Repr()
     requires Valid()
-    requires forall it | it in iters ::allocated(it)
-    ensures Valid()
-    ensures nelems==old(nelems)
-    ensures Model()==old(Model())
-    ensures Iterators()==old(Iterators())
-    ensures list.Length>old(list.Length)
-    ensures c+nelems<list.Length
-    ensures forall it | it in iters ::allocated(it)
-    ensures forall x | x in Repr() - old(Repr()) :: fresh(x)
+    ensures Empty() <==> Model() == []
   {
-      ghost var oldList := ModelAux(list,c,nelems);
-      ghost var oldIterators:=Iterators();
-      var aux: array<int> := new int[2*list.Length+1];
-      assert fresh(aux);
-      assert forall it | it in iters ::{it}!!{this,list,aux}; 
-      var i := 0;
-      while i < nelems
-        decreases nelems-i
-        invariant 0 <= i <= nelems <= list.Length < aux.Length
-        invariant nelems == old(nelems)
-        invariant 0 <= c < list.Length == old(list.Length)
-        invariant ModelAux(aux, 0, i) == ModelAux(list, c, i)
-        invariant ModelAux(list, c, nelems) == oldList
-        invariant forall it |it in iters ::allocated(it)
-        invariant forall it | it in iters ::{it}!!{this,list,aux}
-        invariant Valid() && Iterators()==oldIterators
-      {
-        aux[i] := list[(c+i)%list.Length];
-        i := i+1;
-        assert aux[i-1] == list[(c+i-1)%list.Length];
-        incEnque(aux, 0, old(i));
-        incEnque(list, c, i-1);
-      }
-      assert ModelAux(aux, 0, nelems) == ModelAux(list, c, nelems) == oldList;
-
-      list := aux;
-      c := 0;
-     // assert Iterators()==oldIterators;
-      
-      
+    size == 0
   }
+
+
+  function method Size(): nat
+    reads this, Repr()
+    requires Valid()
+    ensures Size() == |Model()|
+  {
+    size
+  }
+
+
+  function method Front(): int
+    reads this, Repr()
+    requires Valid()
+    requires Model() != []
+    
+    ensures Valid()
+    ensures Front() == Model()[0]
+  {
+    elements[0]
+  }
+
+  method PushFront(x: int)
+    modifies this, Repr()
+    requires Valid()
+    requires forall x | x in Repr() :: allocated(x)
+    
+    ensures Valid()
+    ensures Model() == [x] + old(Model())
+
+    ensures forall x {:trigger x in Repr(), x in old(Repr())} | x in Repr() - old(Repr()) :: fresh(x)
+    ensures fresh(Repr() - old(Repr()))
+    ensures forall x | x in Repr() :: allocated(x)
+
+    ensures Iterators() == old(Iterators())
+    ensures forall it | it in old(iterators) :: old(it.Valid())
+      ==> it.Valid() && old(it.Parent()) == it.Parent() && old(it.Index()) == it.Index();
+  {      
+    if (size == elements.Length) {
+      Grow(elements.Length * 2);
+    }
+    assert size < elements.Length;
+    ShiftRight(0);
+    elements[0] := x;
+    size := size + 1;
+  }
+
+  method PopFront() returns (x: int)
+    modifies this, Repr()
+    requires Valid()
+    requires Model() != []
+    requires forall x | x in Repr() :: allocated(x)
+
+    ensures Valid()
+    ensures [x] + Model() == old(Model())
+
+    ensures forall x {:trigger x in Repr(), x in old(Repr())} | x in Repr() - old(Repr()) :: fresh(x)
+    ensures fresh(Repr() - old(Repr()))
+    ensures forall x | x in Repr() :: allocated(x)
+
+    ensures Iterators() == old(Iterators())
+    ensures forall it | it in old(iterators) :: old(it.Valid()) && old(it.HasNext())
+      ==> it.Valid() && old(it.Parent()) == it.Parent() && old(it.Index()) == it.Index();
+  {
+    x := elements[0];
+    ShiftLeft(0);
+    size := size - 1;
+  }
+
 
   function method Back(): int
     reads this, Repr()
     requires Valid()
     requires Model() != []
+    
     ensures Valid()
     ensures Back() == Model()[|Model()|-1]
-    { 
-      /*if (c+nelems)==0 then list[list.Length-1]
-      else list[(c+nelems-1)%list.Length]*/
-      assert (c+nelems)==0 ==> (c+nelems-1)%list.Length==list.Length-1;
-      list[(c+nelems-1)%list.Length]
-    }
-
-  method PushBack(x: int)
-    modifies Repr()
-    requires Valid()
-    ensures Valid()
-    ensures Model() == old(Model()) + [x]
-    ensures forall x | x in Repr() - old(Repr()) :: fresh(x)
-    ensures forall x | x in Repr() :: allocated(x)
-    ensures Iterators() == old(Iterators())
-    //ensures forall it | it in Iterators() && old(it.Valid()) ::
-    //  it.Valid() // && it.Index() == old(it.Index())
   {
-    ghost var oldList := ModelAux(list,c,nelems);
-    if nelems == list.Length {
-      grow();
-    }
-    assert ModelAux(list, c, nelems) == oldList;
-    
-    list[(c+nelems)%list.Length] := x;
-
-     
-    modulo(c+nelems,list.Length);
-    assert c+nelems<list.Length ==> (c+nelems)%list.Length==c+nelems;
-    assert c+nelems<list.Length ==> list[c..c+nelems]== oldList;
-    assert c+nelems>=list.Length ==> list[c..list.Length]+list[0..(c+nelems)%list.Length]==oldList;
-     
-   
-    nelems := nelems + 1;
-
-    incEnque(list, c, nelems-1);
+    elements[size - 1]
   }
 
-
-lemma modulo(a:int,b:int)
-requires b!=0
-ensures 0<=a<b ==> a/b==0 && a%b==a
-{}
-method PopBack() returns (x: int)
-    modifies Repr()
+  method PopBack() returns (x: int)
+    modifies this, Repr()
     requires Valid()
     requires Model() != []
+    requires forall x | x in Repr() :: allocated(x)
+    
     ensures Valid()
     ensures Model() + [x] == old(Model())
 
-    ensures forall x | x in Repr() - old(Repr()) :: fresh(x)
+    ensures forall x {:trigger x in Repr(), x in old(Repr())} | x in Repr() - old(Repr()) :: fresh(x)
+    ensures fresh(Repr() - old(Repr()))
     ensures forall x | x in Repr() :: allocated(x)
+
     ensures Iterators() == old(Iterators())
-    ensures forall it | it in Iterators() 
-                        && old(it.Valid()) && old(it.Index())<old(|Model()|-1)
-                       :: it.Valid() && it.Index()==old(it.Index())
-    
-
-    { ghost var aux:set<ArrayListIteratorImpl>:=iters;
-      x:=list[(c+nelems-1)%list.Length];
-      nelems:=nelems-1;
-    //assert c+nelems==0 ==> (c+nelems-1)%list.Length==list.Length-1;
-    assert forall it | it in Iterators() &&old(it.Valid()) 
-         && old(it.Index())<old(|Model()|-1):: it.Valid() && it.Index()==old(it.Index());
-     
-   
-
-    
-}
-
-
-function method Front(): int
-    reads this, Repr()
-    requires Valid()
-    requires Model() != []
-    ensures Valid()
-    ensures Front() == Model()[0]
+    ensures forall it | it in old(iterators) :: old(it.Valid()) && old(it.HasNext())
+      ==> it.Valid() && old(it.Parent()) == it.Parent() && old(it.Index()) == it.Index();
   {
-    list[c]
+    assert size > 0;
+    x := elements[size - 1];
+    size := size - 1;
   }
-  method PushFront(x: int)
+
+
+  method PushBack(x: int)
     modifies this, Repr()
     requires Valid()
-    // requires forall x | x in Repr() :: allocated(x)
-    requires forall x | x in Iterators() :: allocated(x)
-    ensures Valid()
-    ensures Model() == [x] + old(Model())
-
-    ensures forall x | x in Repr() - old(Repr()) :: fresh(x)
-    ensures forall x | x in Repr() :: allocated(x)
-
-    ensures Iterators() == old(Iterators())
+    requires forall x | x in Repr() :: allocated(x)
     
-{
-  ghost var oldList := ModelAux(list,c,nelems);
-    if nelems == list.Length {
-      grow();
-    }
-    assert ModelAux(list, c, nelems) == oldList;
-    if (c==0) {c:=list.Length-1;}
-    else {c:=c-1;}
-    list[c]:= x;
-    nelems := nelems + 1;
-    //incEnque(list, c, nelems-1);
-  
-
-}
-
-  method PopFront() returns (x: int)
-    modifies Repr()
-    requires Valid()
-    requires Model() != []
     ensures Valid()
-    ensures [x] + Model() == old(Model())
-    ensures forall x | x in Repr() - old(Repr()) :: fresh(x)
-    ensures forall x | x in Repr() :: allocated(x)
-    ensures Iterators() == old(Iterators())
+    ensures Model() == old(Model()) + [x]
 
+    ensures forall x {:trigger x in Repr(), x in old(Repr())} | x in Repr() - old(Repr()) :: fresh(x)
+    ensures fresh(Repr() - old(Repr()))
+    ensures forall x | x in Repr() :: allocated(x)
+
+    ensures Iterators() == old(Iterators())
+    ensures forall it | it in old(iterators) :: old(it.Valid())
+      ==> it.Valid() && old(it.Parent()) == it.Parent() && old(it.Index()) == it.Index();
   {
-    x := list[c];
-    c := (c+1) % list.Length;
-    nelems := nelems-1;
-    incDeque(list, old(c), old(nelems));
-    // assert ModelAux(list,old(c),f,old(nelems))==[list[old(c)]]+ModelAux(list,(old(c)+1)%list.Length,f,nelems);
+    if (size == elements.Length) {
+      Grow(elements.Length * 2);
+    }
+    assert size < elements.Length;
+    elements[size] := x;
+    size := size + 1;
   }
 
-method Insert(mid: ArrayListIterator, x: int)
+  method Begin() returns (it: ListIterator)
+    modifies this, Repr()
+    requires Valid()
+    requires forall x | x in Repr()::allocated(x)
+    
+    ensures Valid()
+    ensures Model() == old(Model())
+
+    ensures forall x {:trigger x in Repr(), x in old(Repr())} | x in Repr() - old(Repr()) :: fresh(x)
+    ensures fresh(Repr() - old(Repr()))
+    ensures forall x | x in Repr() :: allocated(x)
+
+    ensures fresh(it)
+    ensures it.Valid()
+    ensures it.Parent() == this
+    ensures it.Index() == 0
+    ensures Iterators() == {it} + old(Iterators())
+    ensures forall it | it in old(iterators) :: old(it.Valid())
+      ==> it.Valid() && old(it.Parent()) == it.Parent() && old(it.Index()) == it.Index();
+  {
+    it := new ArrayListIteratorImpl(this);
+    iterators := iterators + { it };
+  }
+
+  // Deletion of mid, next points to the next element (or past-the-end)
+  method Insert(mid: ListIterator, x: int) returns (newt:ListIterator)
+    modifies this, Repr()
+    requires Valid()
+    requires mid.Valid()
+    requires mid.Parent() == this
+    requires mid in Iterators()
+    requires forall x | x in Repr() :: allocated(x)
+
+    ensures Valid()
+    ensures Model() == Seq.Insert(x, old(Model()), old(mid.Index()))
+
+    ensures forall x {:trigger x in Repr(), x in old(Repr())} | x in Repr() - old(Repr()) :: fresh(x)
+    ensures fresh(Repr() - old(Repr()))
+    ensures forall x | x in Repr() :: allocated(x)
+
+    ensures fresh(newt)
+    ensures Iterators() == {newt}+old(Iterators())
+    ensures newt.Valid() && newt.Parent()==this && newt.Index()==old(mid.Index())
+    
+    ensures forall it | it in old(iterators) :: old(it.Valid())
+      ==> it.Valid() && old(it.Parent()) == it.Parent() && old(it.Index()) == it.Index();
+  {
+    var midImpl := mid as ArrayListIteratorImpl;
+   
+    if (size == elements.Length) {
+      Grow(elements.Length * 2);
+    }
+    assert size < elements.Length;
+    assert Model() == old(Model());
+    ShiftRight(midImpl.index);
+    elements[midImpl.index] := x;
+    size := size + 1;
+    assert Model() == Seq.Insert(x, old(Model()), old(mid.Index()));
+
+    newt := midImpl.Copy();
+    iterators := iterators + { newt };
+  }
+
+  // Deletion of mid, next points to the next element (or past-the-end)
+  method Erase(mid: ListIterator) returns (next: ListIterator)
     modifies this, Repr()
     requires Valid()
     requires mid.Valid()
@@ -470,11 +413,121 @@ method Insert(mid: ArrayListIterator, x: int)
     requires mid.HasNext()
     requires mid in Iterators()
     requires forall x | x in Repr() :: allocated(x)
-    ensures Valid()
-    ensures Model() == Seq.Insert(x, old(Model()), old(mid.Index())+1)
-    ensures Iterators() == old(Iterators())
-    ensures forall x | x in Repr() - old(Repr()) :: fresh(x)
-    ensures forall x | x in Repr() :: allocated(x)
     
-   
+    ensures Valid()
+    ensures Model() == Seq.Remove(old(Model()), old(mid.Index()))
+
+    ensures forall x {:trigger x in Repr(), x in old(Repr())} | x in Repr() - old(Repr()) :: fresh(x)
+    ensures fresh(Repr() - old(Repr()))
+    ensures forall x | x in Repr() :: allocated(x)
+
+    ensures fresh(next)
+    ensures Iterators() == {next} + old(Iterators())
+    ensures forall it | it in old(iterators) :: old(it.Valid()) && old(it.HasNext())
+      ==> it.Valid() && old(it.Parent()) == it.Parent() && old(it.Index()) == it.Index();    
+    ensures next.Valid() && next.Parent() == this && next.Index() == mid.Index();
+  {
+    var midImpl := mid as ArrayListIteratorImpl;
+    assert midImpl.index == mid.Index();
+    ShiftLeft(midImpl.index);
+    assert forall j | midImpl.index <= j < size - 1 :: elements[j] == old(elements[j + 1]);
+    assert forall j | 0 <= j < midImpl.index :: elements[j] == old(elements[j]);
+
+    assert elements[..midImpl.index] == old(elements[0..midImpl.index]);
+    assert elements[midImpl.index..size - 1] == old(elements[midImpl.index + 1..size]);
+
+    // assert Seq.Remove(old(elements[..size]), midImpl.index)
+    //         == old(elements[..size])[..midImpl.index] + old(elements[..size])[midImpl.index + 1..size]
+    //         == elements[..midImpl.index] + old(elements[..size])[midImpl.index + 1..]
+    //         == elements[..midImpl.index] + elements[midImpl.index..size - 1]
+    //         == elements[..size - 1];
+
+    // assert elements[..size - 1] == Seq.Remove(old(elements[..size]), midImpl.index);
+    size := size - 1;
+    // assert elements[..size] == Seq.Remove(old(elements[..size]), midImpl.index);
+    // assert Model() == Seq.Remove(old(Model()), midImpl.index);
+    next := midImpl.Copy();
+    iterators := iterators + { next };
+  }
+
+
+  method Grow(newCapacity: nat)
+    requires newCapacity >= elements.Length
+    requires Valid()
+    
+    ensures Valid()
+    ensures Model() == old(Model())
+    ensures this.elements.Length == newCapacity
+
+    ensures forall x {:trigger x in Repr(), x in old(Repr())} | x in Repr() - old(Repr()) :: fresh(x)
+    ensures fresh(Repr() - old(Repr()))
+    
+    ensures Iterators() == old(Iterators())
+    modifies this
+  {
+    var newElements := new int[newCapacity];
+    var i := 0;
+    while (i < size)
+      invariant elements == old(elements)
+      invariant size == old(size)
+      invariant 0 <= i <= size <= elements.Length <= newElements.Length
+      invariant newElements[..i] == elements[..i]
+      invariant newElements[..i] == old(elements)[..i]
+      invariant iterators == old(iterators)
+    {
+      newElements[i] := elements[i];
+      i := i + 1;
+    }
+
+    elements := newElements;
+  }
+
+  method ShiftRight(from: nat)
+    requires 0 <= from <= size < elements.Length
+    modifies this.elements
+    requires Valid()
+    ensures forall j | 0 <= j < from :: elements[j] == old(elements[j]);
+    ensures forall j | from < j <= size :: elements[j] == old(elements[j - 1]);
+    ensures Valid()
+  {
+    ghost var oldElems := elements[..];
+    assert oldElems[..] == old(elements)[..];
+
+    var i := size;
+    while (i > from)
+      invariant from <= i <= size
+      invariant forall j | 0 <= j < i :: elements[j] == oldElems[j]
+      invariant forall j | i < j <= size :: elements[j] == oldElems[j - 1]
+      modifies this.elements
+    {
+      elements[i] := elements[i - 1];
+      i := i - 1;
+    }
+  }
+
+  method ShiftLeft(until: nat)
+    requires 0 <= until < size <= elements.Length
+    requires Valid()
+    ensures forall j | until <= j < size - 1 :: elements[j] == old(elements[j + 1]);
+    ensures forall j | 0 <= j < until :: elements[j] == old(elements[j]);
+    ensures Valid()
+    modifies this.elements
+  {
+    ghost var oldElems := elements[..];
+    assert oldElems[..] == old(elements)[..];
+
+    var i := until;
+    while (i < size - 1)
+      invariant until <= i < size
+      invariant forall j | until <= j < i :: elements[j] == oldElems[j + 1]
+      invariant forall j | i <= j < size :: elements[j] == oldElems[j]
+      invariant forall j | 0 <= j < until :: elements[j] == oldElems[j]
+      modifies this.elements
+    {
+      elements[i] := elements[i + 1];
+      i := i + 1;
+    }
+    assert i == size - 1;
+  }
+
 }
